Heap sort via array apparently translating
It seems that the cause of recent issues is that the monadic translator is
incredibly fragile when it comes to type parameters if the state type needs to
be polymorphic.

Tweak things to check that the type variable is consistent. This code seems to
work with "tvar = ``: 'state``" and "tvar = ``: 'a``" but it does not seem to
work with "tvar = ``: 'el``", which is all a bit mysterious.

basis/heap_sort_monadicScript.sml
@@ -3,19 +3,29 @@
 
   Bit of an experiment, may move to ListProg if useful.
 *)
+
 Theory heap_sort_monadic
 Ancestors
   heap_sort_in_fun ml_translator ml_monad_translator
 Libs
-  preamble ml_monad_translator_interfaceLib
+  preamble ml_translatorLib ml_monad_translator_interfaceLib
 
+(* Part 1. Translator Setup. *)
+
+(* Set up translator to not check subtractions never underflow. *)
+val _ = ml_translatorLib.use_sub_check true;
 
 val _ = set_up_monadic_translator ();
+
+(* The type variable used as parameter to the state type. It seems very
+   important that this is used consistently. Strangely `'a` seems to work (for
+   the current code) though it created problems in a previous iteration. *)
+val tvar = ``: 'a``;
 
 (* Create the data type to handle the references *)
 Datatype:
   state_refs = <|
-                 heap_array : 'a list;
+                 heap_array : ( ^tvar ) list;
                 |>
 End
 
@@ -24,16 +34,18 @@ Datatype:
   state_exn = Fail string | Subscript
 End
 
-val state_type = ``:'el state_refs``;
+val state_type = ``: ( ^tvar ) state_refs``;
 
 val config = local_state_config |>
               with_state state_type |>
               with_exception ``:state_exn`` |>
               with_resizeable_arrays [
-                ("heap_array", ``[] : 'el list``, ``Subscript``, ``Subscript``)
+                ("heap_array", listSyntax.mk_list ([], tvar), ``Subscript``, ``Subscript``)
               ];
 
 val _ = start_translation config;
+
+(* Part 2. Define monadic variants of functions from heap_sort_in_fun theory. *)
 
 Definition heap_insert_larger_monadic_def:
   heap_insert_larger_monadic R sz i x = (if (i = 0n) \/ i * 2 > sz
@@ -270,6 +282,19 @@ Definition heap_pop_all_monadic_def:
     od)
 End
 
+Theorem heap_pop_all_monadic_if_def:
+  heap_pop_all_monadic R sz xs = (if sz = 0n
+    then return xs
+    else do
+      el <- heap_pop_monadic R (sz - 1);
+      heap_pop_all_monadic R (sz - 1) (el :: xs)
+    od
+  )
+Proof
+  Cases_on `sz`
+  \\ simp [heap_pop_all_monadic_def]
+QED
+
 Theorem heap_pop_all_monadic_eq:
   sz <= arr_sz ==>
   ?hp2. (heap_pop_all_monadic R sz xs (st_embed arr_sz hp) =
@@ -287,21 +312,34 @@ Proof
   \\ simp [heap_pop_monadic_eq]
 QED
 
-val run_state_monad_def = 
-  define_run ``: 'a state_refs`` [] "state_monad"
 
-Definition heap_sort_via_monad_def:
-  heap_sort_via_monad R xs = (case xs of
-    [] => []
-  | (x :: _) => (case run_state_monad (do
+(* Part 3. Translation into CakeML AST. *)
+
+val run_init_state_def = define_run state_type [] "init_state";
+
+Definition heap_sort_via_monad_aux1_def:
+  heap_sort_via_monad_aux1 R x xs =
+  (do
       sz <- return (LENGTH xs);
       R2 <- return (\x y. R y x);
       alloc_heap_array sz x;
       heap_add_all_monadic R2 0 xs;
       heap_pop_all_monadic R2 sz [];
-    od) (state_monad [])
-    of (M_success ys) => ys
-      | _ => []
+    od)
+End
+
+Definition heap_sort_via_monad_aux2_def:
+  heap_sort_via_monad_aux2 R x xs =
+  run_init_state (heap_sort_via_monad_aux1 R x xs)
+    (init_state [])
+End
+
+Definition heap_sort_via_monad_def:
+  heap_sort_via_monad R xs = (case xs of
+    [] => []
+  | (x :: _) => (case heap_sort_via_monad_aux2 R x xs of
+    M_success ys => ys
+  | _ => []
   ))
 End
 
@@ -315,32 +353,58 @@ Proof
 QED
 
 Theorem heap_sort_eq:
-  heap_sort R xs = heap_list_sort$heap_sort R xs
+  heap_sort_via_monad R xs = heap_sort R xs
 Proof
-  simp [heap_sort_def, heap_list_sortTheory.heap_sort_def]
+  simp [heap_sort_via_monad_def, heap_sort_def, heap_sort_via_monad_aux2_def,
+    run_init_state_def, heap_sort_via_monad_aux1_def]
   \\ Cases_on `xs` \\ simp []
-  \\ simp [run_state_monad_def, ml_monadBaseTheory.run_def]
+  \\ simp [ml_monadBaseTheory.run_def]
   \\ simp [ml_monadBaseTheory.exc_case_eq, pairTheory.FST_EQ_EQUIV]
   \\ simp [monad_simps, alloc_heap_array_eq]
   \\ simp [heap_add_all_monadic_eq, heap_pop_all_monadic_eq]
 QED
 
-(* Attempt translation of these functions. *)
-
-
-(* Works if the diverging "metis" call is interrupted ??? *)
+fun fix_state_type thm = let
+    val types_in_thm = thm |> concl |> all_atoms
+      |> HOLset.listItems |> map type_of
+      |> map (fn t => fst (strip_fun t) @ [snd (strip_fun t)])
+      |> List.concat
+    val state_matching_types = types_in_thm
+      |> filter (can (match_type state_type))
+      |> HOLset.fromList Type.compare |> HOLset.listItems
+    val substs = map (fn t => match_type t state_type) state_matching_types
+  in case substs of
+    [] => thm
+  | [s] => INST_TYPE s thm
+  | _ => failwith "fix_state_type: multiple!"
+  end
 
 val heap_insert_larger_v_thm = heap_insert_larger_monadic_def
-  |> m_translate;
-
-(* Works if arithmetic is tweaked to avoid "_ - 1" *)
+  |> fix_state_type |> m_translate;
 
 val heap_pop_v_thm = heap_pop_monadic_def
-  |> m_translate;
-
-(* Doesn't work, and other issues prevent definition another way. *)
+  |> fix_state_type |> m_translate;
 
 val heap_pop_all_v_thm = heap_pop_all_monadic_def
-  |> m_translate;
+  |> fix_state_type |> m_translate;
+
+val heap_insert_smaller_v_thm = heap_insert_smaller_monadic_def
+  |> fix_state_type |> m_translate;
+
+val heap_add_v_thm = heap_add_monadic_def
+  |> fix_state_type |> m_translate;
+
+val heap_add_all_v_thm = heap_add_all_monadic_def
+  |> fix_state_type |> m_translate;
+
+val length_v_thm = LENGTH |> translate;
+
+val heap_sort_via_monad_aux1_v_thm = heap_sort_via_monad_aux1_def
+  |> fix_state_type |> m_translate;
+
+val heap_sort_via_monad_aux2_v_thm = heap_sort_via_monad_aux2_def
+  |> fix_state_type |> m_translate_run;
+
+val heap_sort_via_monad_v_thm = heap_sort_via_monad_def |> translate;
 
 
